## 组合数公式

#### $C_n^m=\frac{n!}{m!(n-m)!}$

#### $C_n^m=C_{n-1}^m+C_{n-1}^{m-1}$

#### $C_{n+r+1}^r=\sum_{i=0}^r C_{n+i}^i$

#### $C_n^mC_m^r=C_n^rC_{n-r}^{m-r}$

#### $\sum_{i=0}^n C_n^i=2^n$

#### $\sum_{i=0}^n x^iC_n^i=(x+1)^n$

#### $C_n^0-C_n^1+C_n^2-...±C_n^n=0$

#### $C_n^0+C_n^2+C_n^4...=C_n^1+C_n^3+C_n^5+...=2^{n-1}$

#### $C_{n+m}^r=C_n^0C_m^r+C_n^1C_m^{r-1}+…+C_n^rC_m^0$

#### $mC_n^m=nC_{n-1}^{m-1}$

#### $\sum_{i=1}^n iC_n^i=n2^{n-1}$

#### $\sum_{i=1}^n i^2C_n^i=n(n+1)2^{n-2}$

#### $\sum_{i=0}^n (C_n^i)^2=C_{2n}^n$

#### $\frac{C_n^1}{1}-\frac{C_n^2}{2}+\frac{C_n^3}{3}+…+(-1)^{n-1}\frac{C _n^n}{n} =1 + \frac{1}{2}+ \frac{1}{3}+…+ \frac{1}{n}$

